## Question

If $(x + 1)$ is a factor of $x^3 - 3ax - 3a - 7$, then the value of $a$ is:

**Options:**
- A) 1
- B) –1
- C) 2
- D) –2
- E) 7

## Read the question like a detective
We’re told: “(x + 1) is a factor of x^3 − 3ax − 3a − 7.” We must find a.

Factor means “divides with no leftovers.” Think of sharing candies: if 24 candies are shared among 6 people with none left, 6 is a factor of 24. For polynomials, if (x + 1) is a factor of a polynomial P(x), then when you divide P(x) by (x + 1), the remainder must be 0.

Let’s build that idea from first principles.

---

## Why plugging in x = −1 tells us about the remainder (first principles)
When you divide any polynomial P(x) by (x + 1), you can always write:
```math
P(x) = (x + 1) \cdot Q(x) + R
```
- Q(x) is the quotient (another polynomial),
- R is the remainder. Since we’re dividing by a linear expression (x + 1), the remainder must be a constant (degree < 1).

Now, set x = −1. Then (x + 1) becomes 0:
```math
P(-1) = (0)\cdot Q(-1) + R = R
```
So the remainder equals P(−1). Therefore:
- (x + 1) is a factor of P(x) if and only if P(−1) = 0.

This is the Factor Theorem, derived from the basic division idea, not memorized.

---

## Apply it to our polynomial
Let
```math
P(x) = x^3 - 3ax - 3a - 7.
```
Compute P(−1):
```math
P(-1) = (-1)^3 - 3a(-1) - 3a - 7
      = -1 + 3a - 3a - 7
      = -8.
```
Notice how the 3a and −3a cancel out. The result is −8, which does not depend on a at all.

For (x + 1) to be a factor, we need P(−1) = 0. But we got P(−1) = −8. This can never be 0, no matter what a is.

Conclusion:
- There is no value of a that makes (x + 1) a factor of x^3 − 3ax − 3a − 7.

None of the given options (1, −1, 2, −2, 7) work.

---

## Double-check with a second method: division (to see the “leftover”)
We can do synthetic division by −1 (the root corresponding to x + 1):

Coefficients of P(x): 1, 0, −3a, −3a − 7.

- Bring down 1.
- Multiply by −1 → −1; add to 0 → −1.
- Multiply by −1 → 1; add to −3a → −3a + 1.
- Multiply by −1 → −3a + 1 times −1 → 3a − 1; add to −3a − 7 → −8.

Remainder = −8. So again, not divisible by (x + 1).

---

## A general, structural way to see the impossibility
For a general cubic P(x) = x^3 + bx^2 + cx + d, the condition “(x + 1) is a factor” means:
```math
P(-1) = -1 + b - c + d = 0  \quad \Rightarrow \quad d = c - b + 1.
```
In our problem, b = 0, c = −3a, d = −3a − 7. The condition becomes:
```math
-3a - 7 = (-3a) - 0 + 1 \quad \Rightarrow \quad -3a - 7 = -3a + 1,
```
which simplifies to −7 = 1, a contradiction. So it’s structurally impossible, independent of a.

---

## Likely source of confusion (what if it was x − 1 instead?)
If the question intended “(x − 1) is a factor,” then we’d set P(1) = 0:
```math
P(1) = 1 - 3a - 3a - 7 = -6a - 6 = 0 \Rightarrow a = -1,
```
which matches option B. This suggests the printed factor may have been misstated.

---

## Final answer
- Based strictly on the problem as written: No value of a exists; none of the options is correct.
- If the intended factor was (x − 1): a = −1 (option B).

---

## Conceptual follow-up questions
1. If (x − k) is a factor of a polynomial P(x), why must P(k) = 0? Re-derive using the division-with-remainder idea.
2. For which values of p and q is (x + 1) a factor of x^3 + px + q? Show that P(−1) = 0 forces q = 1.
3. If P(x) = x^3 + bx^2 + cx + d and −1 is a root, derive d in terms of b and c. Then test your formula on a few examples.

## Application questions
- In control systems, the roots of a characteristic polynomial tell you system stability. If a parameter shows up like a in our problem, how would you tune it so a certain root (like −1) is included? What algebraic condition must the coefficients satisfy?
- In digital filters, a factor like (x + 1) corresponds to a zero at −1 (the Nyquist frequency). What must be true about the filter coefficients to place a zero at −1?

## Common misconceptions and reasoning traps
- Thinking a affects P(−1) here: it doesn’t, because the +3a and −3a cancel. Always simplify carefully.
- Plugging the wrong sign: For (x + 1), use x = −1; for (x − 1), use x = 1.
- Forgetting the remainder logic: The remainder when dividing by (x + 1) is exactly P(−1). This comes from the identity P(x) = (x + 1)Q(x) + R, not from rote memory.

## Extension challenges
- Find all real numbers t such that (x + 1) is a factor of x^3 + tx^2 + (t − 4)x + (2t − 3).
- Suppose P(x) = x^4 + ax^3 + bx^2 + cx + d has both (x + 1) and (x − 2) as factors. Derive linear equations linking a, b, c, d and solve for one parameterization.

## Reflective insight
The heart of this topic is the “zeroing” idea: setting x to the value that makes a linear factor zero eliminates the whole product, leaving only the remainder. That’s why evaluating P(k) instantly detects whether (x − k) divides P(x). It’s not a trick; it’s cause-and-effect from the division identity. Once you internalize that, you can handle any factor/root question with confidence.