## Question

The difference between two numbers is $5$ and the difference in their squares is $65$. The larger number is:

## Problem Restated in Simple Words
You have two numbers. The bigger one is 5 more than the smaller one. If you make squares of both numbers and subtract the smaller square from the larger square, you get 65. What is the larger number?

Think of “square” as area: side × side. So the “difference in their squares” is like the difference in the areas of two squares built on the two numbers.

---

## Build the Solution From First Principles

### 1) Set up names and what we know
Let:
- Larger number = $L$
- Smaller number = $S$

We’re told:
```math
L - S = 5
L^2 - S^2 = 65
```

The second line is the “difference of squares.” Rather than using a memorized formula, let’s understand what $L^2 - S^2$ really is.

### 2) Why $L^2 - S^2$ turns into $(L - S)(L + S)$ (area reasoning)
Imagine two squares:
- Big square with side $L$ → area $L^2$
- Small square with side $S$ → area $S^2$

The difference in areas is the border region left when the small square is cut out of the big one. That border can be rearranged into a rectangle with:
- One side equal to the “gap” in sides: $(L - S)$
- The other side equal to the “sum” of sides: $(L + S)$

So the area of that rectangle is:
```math
\text{Area} = (L - S)(L + S)
```
But this area is exactly the difference in the square areas, so:
```math
L^2 - S^2 = (L - S)(L + S)
```

Dimensional check:
- $L, S$ have “length” units
- $L^2, S^2$ have “area” units
- $(L - S)(L + S)$ multiplies length × length = area
- So the equation is dimensionally consistent.

### 3) Use what we know to solve
We already know $L - S = 5$. Substitute into the relation:
```math
L^2 - S^2 = (L - S)(L + S) = 5 \cdot (L + S) = 65
```
So:
```math
L + S = \frac{65}{5} = 13
```

Now we have a simple pair:
```math
L - S = 5
L + S = 13
```

Add the two equations (because adding cancels $S$):
```math
( L - S ) + ( L + S ) = 5 + 13 \Rightarrow 2L = 18 \Rightarrow L = 9
```
Then $S = 13 - L = 13 - 9 = 4$.

So the larger number is 9.

---

## Cross-Check With Pure Algebra (no geometry)
Start again with $S = L - 5$ (because the larger is 5 more).
```math
L^2 - S^2 = 65 \Rightarrow L^2 - (L - 5)^2 = 65
```
Expand $(L - 5)^2$ from first principles: $(L - 5)(L - 5)$
- Multiply term by term: $L \cdot L = L^2$, $L \cdot (-5) = -5L$, $(-5)\cdot L = -5L$, $(-5)\cdot(-5)=25$
- Sum: $L^2 - 10L + 25$

Now substitute:
```math
L^2 - [L^2 - 10L + 25] = 65
L^2 - L^2 + 10L - 25 = 65
10L - 25 = 65
10L = 90
L = 9
```
Same result.

---

## Intuitive “Midpoint” (average) viewpoint
If two numbers differ by 5, they sit symmetrically around their average. Let the average be $m$, and half the gap be $d = 2.5$. Then the numbers are $m + d$ and $m - d$.

Compute the difference of their squares:
```math
(m + d)^2 - (m - d)^2
= [m^2 + 2md + d^2] - [m^2 - 2md + d^2]
= 4md
```
We’re told this equals 65, and $d = 2.5$, so:
```math
4m(2.5) = 65 \Rightarrow 10m = 65 \Rightarrow m = 6.5
```
Therefore, the numbers are $6.5 \pm 2.5$, i.e., 9 and 4. Larger = 9.

---

## Final Answer
```math
\boxed{9}
```

---

## 1) Conceptual Follow-up Questions
- If two numbers differ by $d$, how does the difference of their squares depend on their average? Derive a general expression.
- If $L^2 - S^2$ is fixed, what happens to $L - S$ when $L + S$ increases? Why?
- If $L - S = 5$ but $L^2 - S^2 = 0$, what does that tell you? Is it possible? Why or why not?
- If $L$ and $S$ are negative numbers but still differ by 5, does $L^2 - S^2 = (L - S)(L + S)$ still hold? Explain.

## 2) Real-World Application Questions
- Design: If you increase a square plate’s side from $S$ to $L$, why does the new material needed equal $(L - S)(L + S)$? How could this help estimate material cost quickly?
- Engineering tolerances: If a machine part’s side length changes by a small amount $\delta$, how does the area change approximately? Connect this to $L^2 - S^2 \approx 2S\delta$ when $\delta$ is small.
- Mental math: How can the identity $a^2 - b^2 = (a - b)(a + b)$ help quickly compute 101^2 − 99^2 or 1001^2 − 999^2?

## 3) Common Misconceptions and Traps
- Confusing $a^2 - b^2$ with $(a - b)^2$. Remember:
  - $a^2 - b^2 = (a - b)(a + b)$
  - $(a - b)^2 = a^2 - 2ab + b^2$
- Dropping parentheses: $L^2 - (L - 5)^2$ is not $L^2 - L^2 - 5^2$. Expand carefully.
- Ignoring units/meaning: $L^2 - S^2$ is an “area-like” quantity. $(L - S)(L + S)$ is also area-like. This helps catch algebra slips.

## 4) Extension Challenges
- General case: If $L - S = d$ and $L^2 - S^2 = D$, show that $L + S = D/d$. Then solve for $L$ and $S$ in terms of $d$ and $D$.
- Integer constraint: For which integers $d$ and $D$ does this give integer $L$ and $S$? (Hint: need $D$ divisible by $d$ and parity considerations for $L$ and $S$.)
- Geometry link: Prove $a^2 - b^2 = (a - b)(a + b)$ using a physical rearrangement of shapes (paper cutting).
- Symmetry method: If numbers are $m \pm d$, prove $(m + d)^2 - (m - d)^2 = 4md$ and interpret $4md$ physically.

## 5) Reflective Insight — The Deep “Why”
The difference of two squares measures the “border” you gain when a square grows from side $S$ to side $L$. That border’s area depends on two things at once: the gap $(L - S)$ and the overall scale $(L + S)$. That’s why $L^2 - S^2$ splits naturally into the product $(L - S)(L + S)$. This factorization isn’t a trick; it’s a structural truth about how change in area relates to both the size and the change in side length. Understanding this “why” lets you navigate new problems confidently.