## Question

$(3 \sqrt{2}+2 \sqrt{3})^2+(6-\sqrt{6})^2=$

## Big Idea (start from everyday thinking)
Imagine a square plot whose side length is made of two parts glued together: a “blue” piece plus a “green” piece. The total area is the area of the blue square, plus the green square, plus two rectangles formed between blue and green. That’s why when you square a sum, the “cross-terms” appear.

We’ll use this simple area logic to expand each squared expression, carefully explain why square roots behave the way they do, and then add the results.

## Rebuilding the tools from first principles

### 1) Why does (a + b)^2 become a^2 + 2ab + b^2?
Think of (a + b) as the total length of a side. The area of the square is:
- one square of side a → area a^2,
- one square of side b → area b^2,
- and two rectangles of sides a and b → total area 2ab.

So:
```math
(a + b)^2 = a^2 + 2ab + b^2
```
Algebraically, this is just distributive law:
```math
(a + b)^2 = (a + b)(a + b) = a(a + b) + b(a + b) = a^2 + ab + ba + b^2 = a^2 + 2ab + b^2.
```

Similarly,
```math
(a - b)^2 = a^2 - 2ab + b^2
```
because the two rectangles now subtract instead of add (one is “negative” because of the minus sign).

### 2) Why does √a · √b = √(ab)?
Let x = √a and y = √b. By definition of square root, x^2 = a and y^2 = b.
Then:
```math
(xy)^2 = x^2 y^2 = ab.
```
Since x and y are nonnegative square roots, xy is also nonnegative and must equal the principal square root of ab:
```math
√a · √b = √(ab).
```

## Solve the problem step by step

We need to evaluate:
```math
(3\sqrt{2} + 2\sqrt{3})^2 + (6 - \sqrt{6})^2.
```

### A) Expand (3√2 + 2√3)^2
Use (a + b)^2 = a^2 + 2ab + b^2 with a = 3√2 and b = 2√3.

1) Square each part:
```math
(3\sqrt{2})^2 = 9 \cdot 2 = 18,\quad (2\sqrt{3})^2 = 4 \cdot 3 = 12.
```
2) Cross-term:
```math
2 \cdot (3\sqrt{2}) \cdot (2\sqrt{3}) = 2 \cdot 6 \cdot \sqrt{2}\sqrt{3} = 12\sqrt{6}.
```
So:
```math
(3\sqrt{2} + 2\sqrt{3})^2 = 18 + 12\sqrt{6} + 12 = 30 + 12\sqrt{6}.
```

### B) Expand (6 − √6)^2
Use (a − b)^2 = a^2 − 2ab + b^2 with a = 6 and b = √6.

1) Square each part:
```math
6^2 = 36,\quad (\sqrt{6})^2 = 6.
```
2) Cross-term:
```math
- 2 \cdot 6 \cdot \sqrt{6} = -12\sqrt{6}.
```
So:
```math
(6 - \sqrt{6})^2 = 36 - 12\sqrt{6} + 6 = 42 - 12\sqrt{6}.
```

### C) Add the two results
```math
(30 + 12\sqrt{6}) + (42 - 12\sqrt{6}) = (30 + 42) + (12\sqrt{6} - 12\sqrt{6}) = 72.
```

The √6 terms cancel perfectly—like equal and opposite pulls that balance—leaving just 72.

## Final Answer
```math
72
```

## Sanity check (numerical)
Approximate √2 ≈ 1.414, √3 ≈ 1.732, √6 ≈ 2.449.
- 3√2 + 2√3 ≈ 4.242 + 3.464 = 7.706 → square ≈ 59.39
- 6 − √6 ≈ 3.551 → square ≈ 12.61
Sum ≈ 59.39 + 12.61 ≈ 72.00. Checks out.

---

## Conceptual follow-up questions
1. If you replace 6 with t in (t − √6)^2, for what value of t will the √6 cross-term cancel the cross-term from (3√2 + 2√3)^2?
2. Compare (a + b)^2 + (a − b)^2 with 2(a^2 + b^2). Are they always equal? Why?
3. If (x + y)^2 + (x − y)^2 = 2k, what does that tell you about x^2 + y^2?

## Application questions
- Signal processing: Why do cross-terms matter when adding power from two signals with different phases, and how can designing “opposite cross-terms” cancel interference?
- Structural design: When combining loads that sometimes oppose each other (like wind from different directions), how does “cancellation” show up in the final stress calculation?

## Common misconceptions and traps
- Forgetting that (a + b)^2 ≠ a^2 + b^2. The missing piece is the 2ab cross-term, which represents the two rectangles in the area model.
- Misusing roots: thinking (√a + √b)^2 = √(a + b). It’s not—expanding gives a + b + 2√(ab), which is generally larger than √(a + b) squared.
- Dropping signs in (a − b)^2. The cross-term is negative: −2ab, not +2ab.

## Extension challenges
1. Design numbers u, v, s, t so that (u + v)^2 + (s − t)^2 has all irrational cross-terms cancel. Find one nontrivial example.
2. Generalize: For which real numbers a, b, c, d does (a√2 + b√3)^2 + (c − d√6)^2 simplify to an integer?
3. Prove from first principles (distributive law) the identity:
```math
(a + b)^2 + (a - b)^2 = 2(a^2 + b^2)
```
and interpret it geometrically.

## Reflective insight
The heart of this problem is structure: squaring a sum creates cross-terms that represent interactions between parts. When you combine expressions with symmetric but opposite cross-terms, those interactions cancel, revealing a simpler core (just the sum of the pure squares). Seeing and engineering such cancellations is a powerful mindset in algebra, physics, and engineering—spot the interactions, then control or cancel them.