## Question

Number of terms in the expansion of $(a+b)^2+(a-b)^2$ is

## Start from everyday intuition
- Squaring means “multiply by itself.” So $(a+b)^2$ is $(a+b)(a+b)$.
- When you multiply a sum by a sum, every piece of the first meets every piece of the second. This is just the distributive idea you already use in everyday shopping: cost of (bundle of items) = sum of (cost of each pair of items combined).

We’ll derive everything using only:
- Distributive law: $x(y+z)=xy+xz$.
- Commutative law of multiplication: $xy=yx$.
- Like terms combine (e.g., $ab+ab=2ab$).

## Step-by-step derivation (from first principles)

### 1) Expand $(a+b)^2$
```math
(a+b)^2 = (a+b)(a+b)
        = a\cdot a + a\cdot b + b\cdot a + b\cdot b
        = a^2 + ab + ba + b^2
        = a^2 + 2ab + b^2 \quad\text{(since } ab=ba \text{)}
```

### 2) Expand $(a-b)^2$
```math
(a-b)^2 = (a-b)(a-b)
        = a\cdot a + a\cdot(-b) + (-b)\cdot a + (-b)\cdot(-b)
        = a^2 - ab - ba + b^2
        = a^2 - 2ab + b^2
```

### 3) Add the two expansions
```math
(a+b)^2 + (a-b)^2
= (a^2 + 2ab + b^2) + (a^2 - 2ab + b^2)
= (a^2 + a^2) + (2ab - 2ab) + (b^2 + b^2)
= 2a^2 + 0 + 2b^2
= 2a^2 + 2b^2
```

- The “cross terms” $+2ab$ and $-2ab$ cancel out because they are equal in size and opposite in sign.
- What remains are only two kinds of terms: $a^2$ and $b^2$, each with coefficient 2.

### Answer: number of terms
- In the simplified expression $2a^2 + 2b^2$, there are 2 distinct terms.
- Therefore, the number of terms is 2.

## Quick reality check (numerical test)
Pick $a=3$, $b=1$:
- Left side: $(3+1)^2 + (3-1)^2 = 4^2 + 2^2 = 16 + 4 = 20$.
- Right side: $2a^2 + 2b^2 = 2\cdot 9 + 2\cdot 1 = 18 + 2 = 20$.
They match.

## Visual/area intuition (why the cross terms cancel)
- Think of $(a+b)^2$ as the area of a square with side $(a+b)$. It breaks into four rectangles: $a^2$, two copies of $ab$, and $b^2$.
- $(a-b)^2$ behaves similarly, but the “$ab$-type” pieces appear with a negative sign in algebra. When you add the two squares, the $ab$ parts cancel, leaving only the pure squares: $a^2$ and $b^2$ (each doubled).

## Symmetry viewpoint (deep reason)
- Replace $b$ with $-b$ in $(a+b)^2$: you get $(a-b)^2$.
- Adding a function and its mirror across $b=0$ cancels all terms that change sign with $b$ (odd in $b$), such as $ab$, and keeps those that don’t change sign (even in $b$), such as $a^2$ and $b^2$.
- That’s why only the squares survive.

---

## Final result
```math
(a+b)^2 + (a-b)^2 = 2a^2 + 2b^2
```
Number of terms in the expansion (after simplification): 2.

---

## Conceptual follow-up questions
- If you compute $(a+b)^2 - (a-b)^2$, what survives and why?
- What happens to the number of terms in $(a+b+c)^2 + (a-b-c)^2$ after simplification? Which kinds of terms survive?
- If $b=0$, does the formula still make sense? What does it become?

## Application questions (real-life connections)
- Parallelogram law (physics/geometry): For vectors u and v, $|u+v|^2 + |u-v|^2 = 2(|u|^2 + |v|^2)$. How is this scalar version with $a,b$ a 1D shadow of that?
- Signal processing: Adding a waveform and its inverted version cancels odd components. How does our algebra mirror that?
- Error/variance analysis: Why do cross terms often vanish when averaging symmetric variations around zero?

## Common misconceptions and traps
- Confusing $(a-b)^2$ with $a^2-b^2$. The correct expansion includes the middle term: $(a-b)^2=a^2-2ab+b^2$.
- Counting terms before simplification. Always combine like terms and cancel where possible; then count.
- Forgetting $ab=ba$. Without commutativity, you might incorrectly treat $ab$ and $ba$ as different.

## Extension challenges
- Generalize: Expand and simplify $(a+b)^n + (a-b)^n$ for small $n$ (e.g., $n=3,4$). Which terms cancel? Predict a pattern based on whether $n$ is even or odd.
- For three variables, analyze $(x+y+z)^2 + (x-y-z)^2$. Which cross terms (like $xy, yz, zx$) cancel, and which remain?
- Show directly (using first principles) that $(a+b)^2 - (a-b)^2 = 4ab$, and explain in words why it measures “interaction” between $a$ and $b$.

## Reflective insight
The essence here is symmetry: when you add a quantity and the same quantity with one part flipped (like $b \to -b$), every piece that depends on the direction (sign) of $b$ cancels, while sign-insensitive pieces remain. Algebraically, that’s why cross terms vanish and pure squares stay. Understanding this “even vs odd” idea equips you to predict cancellations in far more complicated expressions.